---
alias: Calc 1 - Rules of Differentiation
---
# Calc 1 - Rules of Differentiation
## The Simple Method of Solving for the Derivative
#maths #calc1

The basic form of the derivative is given by the equation:
$$
f'(x) = \lim_{ h \to 0 } \frac{f(x) - f(x+h)}{h}
$$
This works great for simple problems, but working out the derivative for complex equations becomes exponentially more difficult as you go on. Therefore, it is a lot easier to memorise a number of simple rules for differentiating $f(x)$.

##### Standards Used Throughout the Rest of this Document
- $a$, $b$, $c$, etc. are constants.
- $x$ is a variable.
- $A$, $B$, $C$, etc. are functions of x.
- $u$ is a function of x in substitutions such as the chain rule.

##### Four Function Rules
$$
\begin{align}
&f(x) = A \pm B \\
&f'(x) = A' \pm B'
\end{align}
$$
$$
\begin{align}
&f(x) = A \cdot B \\
&f'(x) = A' \cdot B + B' \cdot A
\end{align}
$$
$$
\begin{align}
&f(x) = \frac{A}{B} \\
&f'(x) = \frac{A' \cdot B - B' \cdot A}{B^2}
\end{align}
$$
##### Power/Constant Rules
$$
\begin{align}
& \frac{d}{dx}x^a = ax^{a+1} \\
& \frac{d}{dx}ax = a \\
& \frac{d}{dx}c = 0
\end{align}
$$
##### Trigonometric Rules
$$
\begin{align}
& \frac{d}{dx}\sin(x) = \cos(x) \\
& \frac{d}{dx}\cos(x) = -\sin(x) \\
\end{align}
$$
We can derive the rules for every other function from these two alone. For instance, we can solve for the tangent rule by using the rules for sine and cosine, and the quotient rule:
$$
\begin{gather}
\frac{d}{dx}\tan x = \frac{d}{dx} \left( \frac{\sin x}{\cos x} \right) \\
\frac{d}{dx}\tan x = \frac{\frac{d}{dx}\sin x \cdot \cos x - \frac{d}{dx}\cos x \cdot \sin x}{\cos^2 x} \\
\frac{d}{dx}\tan x = \frac{\cos^2 x + \sin^2 x}{\cos^2x} \\
\frac{d}{dx}\tan x = \frac{1}{\cos^2 x} = \sec^2(x)
\end{gather}
$$
The flipped rules can also be derived; let's do cosecant as an example:
$$
\begin{gather}
\frac{d}{dx}\csc x = \frac{d}{dx} \left( \frac{1}{\sin x} \right) \\
\frac{d}{dx}\csc x = \frac{\frac{d}{dx} 1 \cdot \sin x - \frac{d}{dx} \sin x \cdot 1}{\sin^2 x}  \\
\frac{d}{dx} \csc x = \frac{-\cos x}{\sin^2 x} = -\cos x \cot x
\end{gather}
$$
Quite a simple solution, actually. Here are the others:
$$
\begin{align}
& \frac{d}{dx}\sec x = \sec x \tan x \\
& \frac{d}{dx}\cot x = -\csc^2 x
\end{align}
$$
The inverse of these functions is also a bit more complicated, but it can be reasoned out from another rule which has limited use cases:
$$
\frac{d}{dx} g'(x) = \frac{1}{f'(g(x))}
$$
where $f(x) = g^{-1}(x)$. Since we know that $\sin^-1 x$ or $\arcsin x$ is the inverse of $\sin x$, meaning that if we set $g(x) = \arcsin x$ then $f(x) = \sin x$ and:
$$
\frac{d}{dx} \arcsin x = \frac{1}{\cos(\arcsin x)}
$$
We also know that $\cos(\arcsin x) = \sqrt{1 - x^2}$, so we can reason out:
$$
\frac{d}{dx} \arcsin x = \frac{1}{\sqrt{ 1 - x^2 }}
$$
The others can be derived in a similar fashion:
$$
\begin{align}
& \frac{d}{dx}\arccos x = -\frac{1}{\sqrt{ 1 - x^2 }} \\
& \frac{d}{dx}\arctan x = \frac{1}{1+x^2} \\ \\
& \frac{d}{dx}\csc^{-1} x = -\frac{1}{|x|\sqrt{ x^2 - 1 }} \\
& \frac{d}{dx}\sec^{-1} x = \frac{1}{|x|\sqrt{ x^2 - 1 }} \\
& \frac{d}{dx}\cot^{-1} x = -\frac{1}{1 + x^2}
\end{align}
$$
##### Logarithmic and Powered Rules
$$
\begin{align}
& \frac{d}{dx} \log_{a} x = \frac{1}{x\ln(a)} \\
& \frac{d}{dx} \ln x = \frac{1}{x} \\
& \frac{d}{dx} c^x = c^x\ln c \\
& \frac{d}{dx} e^x = e^x
\end{align}
$$
##### Chain Rule
This is by far the most important rule of differentiation:
$$
\frac{dy}{dx} = \frac{dy}{du}\cdot \frac{du}{dx}
$$
This means that we can use substitution in our derivatives to make them easier. For instance, when differentiating $y = (x + 1)^2$, we can set $u = x + 1$ and derive as so:
$$
\begin{gather}
\frac{d}{dx} y = \frac{d}{du} y \cdot \frac{d}{dx} u \\
\frac{d}{dx} y = \frac{d}{du}u^2 \cdot \frac{d}{dx} (x+1) \\
\frac{d}{dx} y = 2u \cdot 1 \\
\frac{d}{dx} y = 2(x+1) \cdot 1 \\
\frac{d}{dx} y = 2x + 2
\end{gather}
$$